Common/PDDL_Checker_Utils.thy
@@ -3,58 +3,21 @@ theory PDDL_Checker_Utils
     PDDL_Sema_Supplement
 begin
 
-abbreviation "of_type_x D oT T \<equiv> of_type_impl (ast_domain.STG D) oT T"
-
-abbreviation "wf_domain_x D \<equiv> ast_domain.wf_domain' D (ast_domain.STG D) (ast_domain.mp_constT D)"
-
-abbreviation "wf_problem_x P \<equiv>
-  let D = domain P in
-  ast_problem.wf_problem' P (ast_domain.STG D) (ast_domain.mp_constT D) (ast_problem.mp_objT P)"
+text \<open>This theory used to wrap the generic Formal-PDDL-Semantics executable checker
+  (\<open>ast_domain.STG\<close>, \<open>wf_domain'\<close>, \<open>en_exE2\<close>, \<open>valid_plan_fromE\<close>, \<dots>) in \<open>value\<close>-friendly
+  abbreviations (\<open>wf_domain_x\<close>, \<open>valid_plan_x\<close>, \<dots>) for unit-test probes. That checker layer
+  was renamed/specialized upstream (the generic \<open>ast_domain\<close>/\<open>ast_problem\<close> locales are gone;
+  the executable checker now lives in \<open>ast_cont_domain\<close>/\<open>ast_cont_problem\<close> and the classical
+  path goes through \<open>check_classical_plan\<close>), so those wrappers were removed. Their only uses
+  were already-commented-out probes in \<open>Running_Example.thy\<close>. What remains here are the
+  generic error-revealing helpers.\<close>
 
 (* this just directly displays the first error if applicable *)
 fun reveal_error :: "(unit \<Rightarrow> char list \<Rightarrow> char list) + 'a \<Rightarrow> char list + 'a" where
   "reveal_error (Inl e) = Inl (e () [])" |
   "reveal_error (Inr x) = Inr x"
 
-abbreviation "enab_exec_x P pa s \<equiv>
-  let D = domain P in reveal_error( 
-  ast_problem.en_exE2 P (ast_domain.STG D) (ast_problem.mp_objT P) pa s)"
-
-abbreviation "check_wf_domain_x D \<equiv> reveal_error (
-  check_wf_domain D (ast_domain.STG D) (ast_domain.mp_constT D))"
-
-abbreviation "valid_plan_x P \<pi>s \<equiv>
-  let D = domain P;
-      stg = ast_domain.STG D;
-      obT = ast_problem.mp_objT P;
-      i = ast_problem.I P in
-  reveal_error (ast_problem.valid_plan_fromE P stg obT 1 i \<pi>s)"
-
-(* these are useful for unit tests. You can just do e.g.
-  \<open>lemma "ast_domain.wf_domain some_domain" by (intro wf_domain_intro) eval\<close> *)
-lemmas wf_domain_intro = HOL.iffD1[OF ast_domain.wf_domain'_correct]
-lemmas wf_problem_intro = HOL.iffD1[OF ast_problem.wf_problem'_correct]
-
-lemma (in wf_ast_problem) i_basic: "wm_basic I"
-  using wf_fmla_atom_alt wf_world_model_def wf_I wm_basic_def
-  by metis
-
 lemma reveal_no_error: "reveal_error x = Inr () \<longleftrightarrow> x = Inr()"
   by (cases x; simp)
-
-(* usage:
-  \<open>lemma "ast_problem.valid_plan my_problem my_plan"
-  by (intro valid_plan_intro[OF wf_p1]) eval\<close> *)
-lemma valid_plan_intro:
-  assumes "ast_problem.wf_problem P" "valid_plan_x P \<pi>s = Inr()"
-  shows "ast_problem.valid_plan P \<pi>s"
-proof -
-  from assms have "wm_basic (ast_problem.I P)" using wf_ast_problem.intro wf_ast_problem.i_basic by simp
-  with assms have "ast_problem.valid_plan_from P (ast_problem.I P) \<pi>s"
-    using ast_problem.valid_plan_fromE_return_iff' reveal_no_error by simp
-  thus ?thesis using ast_problem.valid_plan_def by simp
-qed
-
-
 
 end
