SMLCodebase/examples/domain.pddl
@@ -1,0 +1,41 @@
+;; Transcription of Running_Example.thy `my_domain` (Helmert 2009, modified):
+;; type hierarchy, Either-typed parameters, multiple inheritance (Batmobile),
+;; circular type graph (R/L), disjunctive preconditions.
+(define (domain running-example)
+  (:requirements :strips :typing :disjunctive-preconditions)
+  (:types
+    City Movable - object
+    Vehicle Parcel - Movable
+    Car Train - Vehicle
+    R - L
+    L - R
+    Batmobile - Car
+    Batmobile - Train)
+  (:constants A B C D E F G - City)
+  (:predicates
+    (at ?m - Movable ?c - City)
+    (in ?p - Parcel ?v - (either Car Train))
+    (road ?x - City ?y - City)
+    (rails ?x - City ?y - City))
+
+  (:action drive
+    :parameters (?c - Car ?from - City ?to - City)
+    :precondition (and (at ?c ?from)
+                       (or (road ?from ?to) (road ?to ?from)))
+    :effect (and (at ?c ?to) (not (at ?c ?from))))
+
+  (:action choochoo
+    :parameters (?t - Train ?from - City ?to - City)
+    :precondition (and (at ?t ?from)
+                       (or (rails ?from ?to) (rails ?to ?from)))
+    :effect (and (at ?t ?to) (not (at ?t ?from))))
+
+  (:action load
+    :parameters (?what - Parcel ?where - City ?into - (either Car Train))
+    :precondition (and (at ?into ?where) (at ?what ?where))
+    :effect (and (in ?what ?into) (not (at ?what ?where))))
+
+  (:action unload
+    :parameters (?what - Parcel ?from - (either Car Train) ?where - City)
+    :precondition (and (at ?from ?where) (in ?what ?from))
+    :effect (and (at ?what ?where) (not (in ?what ?from)))))
