SMLCodebase/examples/problem.pddl
@@ -1,0 +1,17 @@
+;; Transcription of Running_Example.thy `my_problem`.
+;; (batmobile is deliberately absent from init, as in the theory.)
+(define (problem running-example-1)
+  (:domain running-example)
+  (:objects
+    c1 c2 c3 - Car
+    t - Train
+    p1 p2 - Parcel
+    batmobile - Batmobile)
+  (:init
+    (at c1 A) (at c2 B) (at c3 G)
+    (at t E)
+    (at p1 C) (at p2 F)
+    (road A D) (road B D) (road C D)
+    (rails D E)
+    (road E F) (road F G) (road G E))
+  (:goal (and (at p1 G) (at p2 E))))
